\documentclass[12pt]{article}
\usepackage{amsmath}
\usepackage{amssymb}
\usepackage[letterpaper,top=1in,bottom=1.25in,left=0.75in,right=0.75in,centering]{geometry}
%\usepackage{fancyhdr}
\usepackage{enumerate}
%\usepackage{lastpage}
\usepackage{multicol}
\usepackage{graphicx}

%\reversemarginpar

%\pagestyle{fancy}
%\cfoot{}
%\lhead{Math 1560}\chead{Test \# 1}\rhead{May 18th, 2017}
%\rfoot{Total: 10 points}
%\chead{{\bf Name:}}
\newcommand{\points}[1]{\marginpar{\hspace{24pt}[#1]}}
\newcommand{\skipline}{\vspace{12pt}}
%\renewcommand{\headrulewidth}{0in}
\headheight 30pt

\newcommand{\di}{\displaystyle}
\newcommand{\abs}[1]{\lvert #1\rvert}
\newcommand{\len}[1]{\lVert #1\rVert}
\renewcommand{\i}{\mathbf{i}}
\renewcommand{\j}{\mathbf{j}}
\renewcommand{\k}{\mathbf{k}}
\newcommand{\R}{\mathbb{R}}
\newcommand{\aaa}{\mathbf{a}}
\newcommand{\bbb}{\mathbf{b}}
\newcommand{\ccc}{\mathbf{c}}
\newcommand{\dotp}{\boldsymbol{\cdot}}
\newcommand{\bbm}{\begin{bmatrix}}
\newcommand{\ebm}{\end{bmatrix}}                   
                  
\begin{document}


\author{Instructor: Sean Fitzpatrick}
\thispagestyle{empty}
\begin{center}
\emph{University of Lethbridge}\\
Department of Mathematics and Computer Science\\
{\bf MATH 1565 - Tutorial \#2 Solutions}\\
\end{center}
%\skipline \skipline \skipline \noindent \skipline
%Last Name:\underline{\hspace{350pt}}\\
%\skipline
%First Name:\underline{\hspace{348pt}}\\
%\skipline
%Student Number:\underline{\hspace{322pt}}\\
%\skipline

\begin{enumerate}
 \item  Evaluate the limit $\di \lim_{x\to 0}\frac{1-\cos(5t)}{\sin^2(3t)}$.
 
 We note that by direct substitution, the limit is of $0/0$ form. Since $1-\cos^2\theta=\sin^2\theta$, we have
 \begin{align*}
 \lim_{x\to 0}\frac{1-\cos(5t)}{\sin^2(3t)} & = \lim_{x\to 0}\frac{1-\cos(5t)}{\sin^2(3t)}\cdot\frac{1+\cos(5t)}{1+\cos(5t)} = \lim_{x\to 0}\frac{1-\cos^2(5t)}{\sin^2(3t)(1+\cos(5t)}\\
 & = \lim_{x\to 0}\frac{1}{1+\cos(5t)}\cdot \left(\frac{\sin(5t)}{\sin(3t)}\right)^2 = \lim_{x\to 0}\frac{1}{1+\cos(5t)}\left(\frac{5}{3}\cdot \frac{\sin(5t)}{5t}\cdot \frac{3t}{\sin(3t)}\right)^2\\
 & = \frac{1}{1+1}\left(\frac{5}{3}(1)(1)\right)^2 = \frac{25}{18}.
 \end{align*}
 
 \medskip
 
 \item Evaluate the limit $\di \lim_{x\to 2}\frac{x^3-8}{x^4-16}$.
 
 Trying direct substitution, we see that the limit is of form $0/0$, so we evaluate by factoring:
 \begin{align*}
 \lim_{x\to 2}\frac{x^3-8}{x^4-16} & = \lim_{x\to 2}\frac{(x-2)(x^2+2x+4)}{(x-2)(x+2)(x^2+4)}\\
 & = \lim_{x\to 2}\frac{x^2+2x+4}{(x+2)(x^2+4)} = \frac{2^2+2^2+4}{(2+2)(2^2+4)} = \frac{12}{32} = \frac{3}{8}.
 \end{align*}
 
 \medskip
 
 \item Evaluate the limit $\di \lim_{x\to -\infty}\frac{\sqrt{x^2+2}}{3x-4}$.
 
 This time, we see that we're in an ``$\infty/\infty$'' situation, which also requires further investigation. We find:
 \begin{align*}
 \lim_{x\to -\infty}\frac{\sqrt{x^2+2}}{3x-4}& = \lim_{x\to -\infty}\frac{\sqrt{x^2(1+2/x^2)}}{x(3-4/x)} = \lim_{x\to -\infty}\frac{\sqrt{x^2}\sqrt{1+2/x^2}}{x(3-4/x)}\\
 & = \lim_{x\to -\infty}\frac{-x\sqrt{1+2/x^2}}{x(3-4/x)}= \lim_{x\to -\infty}\frac{-\sqrt{1+2/x^2}}{3-4/x}\\
 & = \frac{-\sqrt{1+0}}{3-0} = -\frac{1}{3}.
 \end{align*}
 \textbf{Note:} Recall that $\sqrt{x^2} = \abs{x}$. Since $x\to -\infty$, we can assume that $x<0$, and thus $\sqrt{x^2}=-x$, which is why we have $-x$ in the numerator in the second line above.
\end{enumerate}

\end{document}