\documentclass[12pt]{article}
\usepackage{amsmath}
\usepackage{amssymb}
\usepackage[letterpaper,top=0.75in,bottom=0.75in,left=0.75in,right=0.75in,centering]{geometry}
%\usepackage{fancyhdr}
\usepackage{enumerate}
%\usepackage{lastpage}
\usepackage{multicol}
\usepackage{graphicx}

%\reversemarginpar

%\pagestyle{fancy}
%\cfoot{}
%\lhead{Math 1560}\chead{Test \# 1}\rhead{May 18th, 2017}
%\rfoot{Total: 10 points}
%\chead{{\bf Name:}}
\newcommand{\points}[1]{\marginpar{\hspace{24pt}[#1]}}
\newcommand{\skipline}{\vspace{12pt}}
%\renewcommand{\headrulewidth}{0in}
\headheight 30pt

\newcommand{\di}{\displaystyle}
\newcommand{\abs}[1]{\lvert #1\rvert}
\newcommand{\len}[1]{\lVert #1\rVert}
\renewcommand{\i}{\mathbf{i}}
\renewcommand{\j}{\mathbf{j}}
\renewcommand{\k}{\mathbf{k}}
\newcommand{\R}{\mathbb{R}}
\newcommand{\aaa}{\mathbf{a}}
\newcommand{\bbb}{\mathbf{b}}
\newcommand{\ccc}{\mathbf{c}}
\newcommand{\dotp}{\boldsymbol{\cdot}}
\newcommand{\bbm}{\begin{bmatrix}}
\newcommand{\ebm}{\end{bmatrix}}                   
                  
\begin{document}


\author{Instructor: Sean Fitzpatrick}
\thispagestyle{empty}
\vglue1cm
\begin{center}
{\bf MATH 1565 - Tutorial \#5 Solutions}\\
\end{center}

Determine $f'(x)$ for the following functions: 
\begin{enumerate}
 \item   $f(x)= x^{38} + 4 \ln(x) -3e^{x} + \pi^{3000}$.

\bigskip

Using the sum and constant rules,
\[
f'(x) = 38x^{37}+4\cdot\frac{1}{x}-3e^x.
\]

\bigskip

 \item $f(x) =x^5e^{x}\tan(x)$.
 
\bigskip

Using the product rule (twice),
\[
f'(x) = 5x^4e^x\tan(x)+x^5e^x\tan(x)+x^5e^x\sec^2(x).
\]

\bigskip

 
 \item $f(x) = \cot(x)$. (Write $\cot(x)=\dfrac{\cos(x)}{\sin(x)}$ and use the quotient rule.)
 
\bigskip

Using the quotient rule,
\begin{align*}
f'(x) &= \frac{\left(\frac{d}{dx}(\cos(x))\right)\sin(x)-\cos(x)\frac{d}{dx}(\sin(x))}{\sin^2(x)}\\
& = \frac{-\sin^2(x)-\cos^2(x)}{\sin^2(x)}\\
& = \frac{-1}{\sin^2(x)} = -\csc^2(x).
\end{align*}
 
 \bigskip
 
 
 \item  $f(x) = \cos(e^{x}+ 13x^{11}-\sin(x))$. 
 
\bigskip

Using the chain rule,
\begin{align*}
f'(x) & = -\sin(e^{x}+ 13x^{11}-\sin(x))\frac{d}{dx}(e^{x}+ 13x^{11}-\sin(x))\\
& = -\sin(e^{x}+ 13x^{11}-\sin(x))(e^x+13(11x^{10})-\cos(x))
\end{align*}
\end{enumerate}
\end{document}