\documentclass[12pt]{article}
\usepackage{amsmath}
\usepackage{amssymb}
\usepackage[letterpaper,top=1in,bottom=1.25in,left=0.75in,right=0.75in,centering]{geometry}
%\usepackage{fancyhdr}
\usepackage{enumerate}
%\usepackage{lastpage}
\usepackage{multicol}
\usepackage{graphicx}

\reversemarginpar

%\pagestyle{fancy}
%\cfoot{}
%\lhead{Math 1560}\chead{Test \# 1}\rhead{May 18th, 2017}
%\rfoot{Total: 10 points}
%\chead{{\bf Name:}}
\newcommand{\points}[1]{\marginpar{\hspace{24pt}[#1]}}
\newcommand{\skipline}{\vspace{12pt}}
%\renewcommand{\headrulewidth}{0in}
\headheight 30pt

\newcommand{\di}{\displaystyle}
\newcommand{\abs}[1]{\lvert #1\rvert}
\newcommand{\len}[1]{\lVert #1\rVert}
\renewcommand{\i}{\mathbf{i}}
\renewcommand{\j}{\mathbf{j}}
\renewcommand{\k}{\mathbf{k}}
\newcommand{\R}{\mathbb{R}}
\newcommand{\aaa}{\mathbf{a}}
\newcommand{\bbb}{\mathbf{b}}
\newcommand{\ccc}{\mathbf{c}}
\newcommand{\dotp}{\boldsymbol{\cdot}}
\newcommand{\bbm}{\begin{bmatrix}}
\newcommand{\ebm}{\end{bmatrix}}                   
                  
\begin{document}


%\author{Instructor: Sean Fitzpatrick}
\thispagestyle{empty}
\begin{center}
\emph{University of Lethbridge}\\
Department of Mathematics and Computer Science\\
{\bf MATH 1565 - Quiz \#3 Solution}\\
\end{center}
\thispagestyle{empty}
\begin{enumerate}
 \item Determine the equation of the tangent line to the curve
 \[
 (x^2+y^2+y)^2=x^2+y^2
 \]
 at the point $(1,0)$.
% \end{enumerate}
\end{enumerate}

Taking the derivative of both sides of the equation with respect to $x$, we have
\[
2(x^2+y^2+y)\left(2x+2y\frac{dy}{dx}+\frac{dy}{dx}\right)=2x+2y\frac{dy}{dx}.
\]
Having taken the derivative, we can put in $x=1$, $y=0$, giving us
\[
2(1+0+0)\left(2+0+\frac{dy}{dx}\right)=2(1)+0,
\]
so $2(2+dy/dx)=2$, giving us $2+dy/dx=1$, so  $\dfrac{dy}{dx}=-1$.

With the slope $m=-1$ and point $(1,0)$ we obtain the equation
\[
y-0=-1(x-1) \text{ or } y=-x+1
\]
for the tangent line.

\bigskip

\textbf{Note:} it was not necessary to solve for $\dfrac{dy}{dx}$ in terms of $x$ and $y$ before putting  in the given values, but if you did, you should get:
\[
4y(x^2+y^2+y)\frac{dy}{dx}+2(x^2+y^2+y)\frac{dy}{dx}+4x(x^2+y^2+y)=2x+2y\frac{dy}{dx},
\]
so
\[
\frac{dy}{dx} = \frac{2x-4x^3-4xy^2-4xy}{4x^2y+4y^3+6y^2+2x^2}.
\]
\end{document}